concurrency/scache/CacheOps.i.dfy
@@ -517,8 +517,7 @@ module CacheOps(aio: AIO(CacheAIOParams, CacheIfc, CacheSSM)) {
     }
   }
 
-  method get_free_page(shared cache: Cache, linear inout localState: LocalState,
-      new_status: uint8)
+  method get_free_page(shared cache: Cache, linear inout localState: LocalState)
   returns (
     cache_idx: uint64,
     glinear m: T.Token,
@@ -526,16 +525,11 @@ module CacheOps(aio: AIO(CacheAIOParams, CacheIfc, CacheSSM)) {
   )
   requires cache.Inv()
   requires old_localState.WF()
-  requires new_status == flag_exc_accessed_reading_clean
-        || new_status == flag_accessed_reading_clean
   ensures localState.WF()
   ensures
       && 0 <= cache_idx as int < CACHE_SIZE as int
       && m.loc == cache.status[cache_idx].rwlock_loc
-      && (new_status == flag_exc_accessed_reading_clean ==>
-           m.val == RwLock.ReadHandle(RwLock.ReadPending))
-      && (new_status == flag_accessed_reading_clean ==>
-           m.val == RwLock.ReadHandle(RwLock.ReadObtained(-1)))
+      && m.val == RwLock.ReadHandle(RwLock.ReadPending)
       && handle.is_handle(cache.key(cache_idx as int))
       && handle.CacheEmptyHandle?
   ensures localState.t == old_localState.t
@@ -569,10 +563,7 @@ module CacheOps(aio: AIO(CacheAIOParams, CacheIfc, CacheSSM)) {
         && 0 <= cache_idx as int < CACHE_SIZE as int
         && m_opt.glSome?
         && m_opt.value.loc == cache.status[cache_idx].rwlock_loc
-        && (new_status == flag_exc_accessed_reading_clean ==>
-             m_opt.value.val == RwLock.ReadHandle(RwLock.ReadPending))
-        && (new_status == flag_accessed_reading_clean ==>
-             m_opt.value.val == RwLock.ReadHandle(RwLock.ReadObtained(-1)))
+        && m_opt.value.val == RwLock.ReadHandle(RwLock.ReadPending)
         && handle_opt.glSome?
         && handle_opt.value.is_handle(cache.key(cache_idx as int))
         && handle_opt.value.CacheEmptyHandle?
@@ -591,10 +582,7 @@ module CacheOps(aio: AIO(CacheAIOParams, CacheIfc, CacheSSM)) {
           && 0 <= cache_idx as int < CACHE_SIZE as int
           && m_opt.glSome?
           && m_opt.value.loc == cache.status[cache_idx].rwlock_loc
-          && (new_status == flag_exc_accessed_reading_clean ==>
-               m_opt.value.val == RwLock.ReadHandle(RwLock.ReadPending))
-          && (new_status == flag_accessed_reading_clean ==>
-               m_opt.value.val == RwLock.ReadHandle(RwLock.ReadObtained(-1)))
+          && m_opt.value.val == RwLock.ReadHandle(RwLock.ReadPending)
           && handle_opt.glSome?
           && handle_opt.value.is_handle(cache.key(cache_idx as int))
           && handle_opt.value.CacheEmptyHandle?
@@ -603,7 +591,7 @@ module CacheOps(aio: AIO(CacheAIOParams, CacheIfc, CacheSSM)) {
 
         dispose_glnone(m_opt);
         dispose_glnone(handle_opt);
-        success, m_opt, handle_opt := cache.status_atomic(cache_idx).try_alloc(new_status);
+        success, m_opt, handle_opt := cache.status_atomic(cache_idx).try_alloc();
 
         i := i + 1;
       }
@@ -652,8 +640,7 @@ module CacheOps(aio: AIO(CacheAIOParams, CacheIfc, CacheSSM)) {
 
     if cache_idx == NOT_MAPPED {
       glinear var r, handle;
-      cache_idx, r, handle := get_free_page(cache, inout localState,
-          flag_exc_accessed_reading_clean);
+      cache_idx, r, handle := get_free_page(cache, inout localState);
 
       glinear var read_stub;
       glinear var read_ticket_opt;
@@ -1019,14 +1006,14 @@ module CacheOps(aio: AIO(CacheAIOParams, CacheIfc, CacheSSM)) {
     var done := false;
     while !done
     decreases *
+    invariant localState.WF()
     {
       var cache_idx := atomic_index_lookup_read(
           cache.cache_idx_of_page_atomic(disk_idx), disk_idx as nat);
       if cache_idx == NOT_MAPPED {
       } else {
         glinear var m, handle;
-        cache_idx, m, handle := get_free_page(cache, inout localState,
-            flag_accessed_reading_clean);
+        cache_idx, m, handle := get_free_page(cache, inout localState);
 
         glinear var read_ticket_opt;
         glinear var CacheEmptyHandle(_, cache_empty, idx, data) := handle;
@@ -1052,6 +1039,13 @@ module CacheOps(aio: AIO(CacheAIOParams, CacheIfc, CacheSSM)) {
                   data));
         } else {
           dispose_glnone(cache_empty_opt);
+
+          m := cache.status_atomic(cache_idx).clear_exc_bit_during_load_phase(m);
+
+          write_cell(
+            cache.disk_idx_of_entry_ptr(cache_idx),
+            inout idx,
+            disk_idx as int64);
 
           disk_read_async(cache, inout localState,
               disk_idx, cache_idx, cache.data_ptr(cache_idx),
